NuPrime.thy
@@ -483,6 +483,12 @@ syntax "_codeblock_noarg_exp_" :: "idt \<Rightarrow> logic \<Rightarrow> bool"  
 syntax "_codeblock_" :: "idt \<Rightarrow> logic \<Rightarrow> bool" ("\<^bold>c\<^bold>o\<^bold>d\<^bold>e\<^bold>b\<^bold>l\<^bold>o\<^bold>c\<^bold>k _ \<^bold>f\<^bold>o\<^bold>r \<^bold>a\<^bold>r\<^bold>g\<^bold>u\<^bold>m\<^bold>e\<^bold>n\<^bold>t\<^bold>s '\<open>_'\<close>" [100,0] 3)
 syntax "_codeblock_noarg_" :: "idt \<Rightarrow> bool" ("\<^bold>c\<^bold>o\<^bold>d\<^bold>e\<^bold>b\<^bold>l\<^bold>o\<^bold>c\<^bold>k _ \<^bold>w\<^bold>i\<^bold>t\<^bold>h\<^bold>o\<^bold>u\<^bold>t \<^bold>a\<^bold>r\<^bold>g\<^bold>u\<^bold>m\<^bold>e\<^bold>n\<^bold>t" [100] 3)
 
+(* definition CodeBlock' :: " ('a::lrep) state \<Rightarrow> ('b::lrep) state => ('b \<longmapsto> 'a) \<Rightarrow> bool" where
+  CodeBlock'_def: "CodeBlock' stat arg prog \<longleftrightarrow> (bind arg prog = stat \<and> stat \<noteq> PartialCorrect)"
+
+lemma accept_proc'': "\<^bold>p\<^bold>e\<^bold>n\<^bold>d\<^bold>i\<^bold>n\<^bold>g g \<^bold>o\<^bold>n s \<^bold>r\<^bold>e\<^bold>s\<^bold>u\<^bold>l\<^bold>t\<^bold>s \<^bold>i\<^bold>n T \<Longrightarrow> (\<And>s'. CodeBlock' s' s g \<Longrightarrow> \<^bold>c\<^bold>u\<^bold>r\<^bold>r\<^bold>e\<^bold>n\<^bold>t s' \<^bold>r\<^bold>e\<^bold>s\<^bold>u\<^bold>l\<^bold>t\<^bold>s \<^bold>i\<^bold>n T)" *)
+  
+
 attribute_setup show_codeblock_expression =  \<open>
   Scan.lift (Parse.$$$ "=" |-- ((Args.$$$ "false" >> K false) || (Args.$$$ "true" >> K true)) >>
     (Thm.declaration_attribute o K o Config.put_generic NuConfig.show_codeblock_expression))\<close>
@@ -572,6 +578,8 @@ theorem accept_proc' : "\<medium_left_bracket> \<And>s. CodeBlock s a S f \<Long
   CodeBlock s' a S (f \<nuInstrComp> g) \<Longrightarrow> (\<^bold>c\<^bold>u\<^bold>r\<^bold>r\<^bold>e\<^bold>n\<^bold>t s' \<^bold>r\<^bold>e\<^bold>s\<^bold>u\<^bold>l\<^bold>t\<^bold>s \<^bold>i\<^bold>n T)" for  s' :: "('c::lrep) state"
   unfolding PropBlock_def CodeBlock_def instr_comp_def CurrentConstruction_def PendingConstruction_def bind_def
   by (auto 4 4)
+
+
 
 lemma codeblock_export: "PROP Pure.prop (\<And>s. CodeBlock s a T f \<Longrightarrow> PROP C) \<Longrightarrow> PROP Pure.prop (\<And>s. CodeBlock s a T (f \<nuInstrComp> g) \<Longrightarrow> PROP C)"
   unfolding CodeBlock_def prop_def instr_comp_def proof -
